<math xmlns="http://www.w3.org/1998/Math/MathML" display="block"><mo>如果</mo><mi>a</mi><mo>=</mo><mi>b</mi><mo>，那么</mo><mi>a</mi><mo>+</mo><mi>c</mi><mo>=</mo><mi>b</mi><mo>+</mo><mi>c</mi></math>

<math xmlns="http://www.w3.org/1998/Math/MathML" display="block"><mo>如果</mo><mi>a</mi><mo>=</mo><mi>b</mi><mo>，那么</mo><mi>a</mi><mo>−</mo><mi>c</mi><mo>=</mo><mi>b</mi><mo>−</mo><mi>c</mi></math>

<math xmlns="http://www.w3.org/1998/Math/MathML" display="block"><mo>如果</mo><mi>a</mi><mo>=</mo><mi>b</mi><mo>，那么</mo><mi>a</mi><mo>×</mo><mi>c</mi><mo>=</mo><mi>b</mi><mo>×</mo><mi>c</mi></math>

<math xmlns="http://www.w3.org/1998/Math/MathML" display="block"><mo>如果</mo><mi>a</mi><mo>=</mo><mi>b</mi><mo>，那么</mo><mfrac><mi>a</mi><mi>c</mi></mfrac><mo>=</mo><mfrac><mi>b</mi><mi>c</mi></mfrac><mo stretchy="false">(</mo><mi>c</mi><mo>≠</mo><mn>0</mn><mo stretchy="false">)</mo></math>