## 二元一次

### 代入法

解：

<math xmlns="http://www.w3.org/1998/Math/MathML" display="block"><mrow data-mjx-texclass="INNER"><mo data-mjx-texclass="OPEN">{</mo><mtable columnspacing="1em" rowspacing="4pt"><mtr><mtd><mi>a</mi><mo>−</mo><mi>b</mi><mo>=</mo><mn>1</mn><mrow><mo>①</mo></mrow></mtd></mtr><mtr><mtd><mi>a</mi><mo>+</mo><mi>b</mi><mo>=</mo><mn>3</mn><mrow><mo>②</mo></mrow></mtd></mtr></mtable><mo data-mjx-texclass="CLOSE" fence="true" stretchy="true" symmetric="true"></mo></mrow></math>

由 ①，得

<math xmlns="http://www.w3.org/1998/Math/MathML" display="block"><mi>a</mi><mo>=</mo><mi>b</mi><mo>+</mo><mn>1</mn><mrow><mo>③</mo></mrow></math>

将 ③ 代入 ②，得

<math xmlns="http://www.w3.org/1998/Math/MathML" display="block"><mtable columnalign="right left right left right left right left right left right left" columnspacing="0em 2em 0em 2em 0em 2em 0em 2em 0em 2em 0em" rowspacing="3pt" displaystyle="true"><mtr><mtd><mo stretchy="false">(</mo><mi>b</mi><mo>+</mo><mn>1</mn><mo stretchy="false">)</mo><mo>+</mo><mi>b</mi><mo>=</mo><mn>3</mn></mtd></mtr><mtr><mtd><mi>b</mi><mo>+</mo><mn>1</mn><mo>+</mo><mi>b</mi><mo>=</mo><mn>3</mn></mtd></mtr><mtr><mtd><mn>2</mn><mi>b</mi><mo>=</mo><mn>2</mn></mtd></mtr><mtr><mtd><mi>b</mi><mo>=</mo><mn>1</mn></mtd></mtr></mtable></math>

将 <math xmlns="http://www.w3.org/1998/Math/MathML"><mi>b</mi><mo>=</mo><mn>1</mn></math> 代入 ③，得

<math xmlns="http://www.w3.org/1998/Math/MathML" display="block"><mtable columnalign="right left right left right left right left right left right left" columnspacing="0em 2em 0em 2em 0em 2em 0em 2em 0em 2em 0em" rowspacing="3pt" displaystyle="true"><mtr><mtd><mi>a</mi><mo>=</mo><mn>1</mn><mo>+</mo><mn>1</mn></mtd></mtr><mtr><mtd><mi>a</mi><mo>=</mo><mn>2</mn></mtd></mtr></mtable></math>

所以这个方程组的解是

<math xmlns="http://www.w3.org/1998/Math/MathML" display="block"><mrow data-mjx-texclass="INNER"><mo data-mjx-texclass="OPEN">{</mo><mtable columnspacing="1em" rowspacing="4pt"><mtr><mtd><mi>a</mi><mo>=</mo><mn>2</mn></mtd></mtr><mtr><mtd><mi>b</mi><mo>=</mo><mn>1</mn></mtd></mtr></mtable><mo data-mjx-texclass="CLOSE" fence="true" stretchy="true" symmetric="true"></mo></mrow></math>

---

### 加减法

解：

<math xmlns="http://www.w3.org/1998/Math/MathML" display="block"><mrow data-mjx-texclass="INNER"><mo data-mjx-texclass="OPEN">{</mo><mtable columnspacing="1em" rowspacing="4pt"><mtr><mtd><mi>a</mi><mo>−</mo><mi>b</mi><mo>=</mo><mn>1</mn><mrow><mo>①</mo></mrow></mtd></mtr><mtr><mtd><mi>a</mi><mo>+</mo><mi>b</mi><mo>=</mo><mn>3</mn><mrow><mo>②</mo></mrow></mtd></mtr></mtable><mo data-mjx-texclass="CLOSE" fence="true" stretchy="true" symmetric="true"></mo></mrow></math>

① + ②，得

<math xmlns="http://www.w3.org/1998/Math/MathML" display="block"><mtable columnalign="right left right left right left right left right left right left" columnspacing="0em 2em 0em 2em 0em 2em 0em 2em 0em 2em 0em" rowspacing="3pt" displaystyle="true"><mtr><mtd><mn>2</mn><mi>a</mi><mo>=</mo><mn>4</mn></mtd></mtr><mtr><mtd><mi>a</mi><mo>=</mo><mn>2</mn></mtd></mtr></mtable></math>

将 <math xmlns="http://www.w3.org/1998/Math/MathML"><mi>a</mi><mo>=</mo><mn>2</mn></math> 代入 ①，得

<math xmlns="http://www.w3.org/1998/Math/MathML" display="block"><mtable columnalign="right left right left right left right left right left right left" columnspacing="0em 2em 0em 2em 0em 2em 0em 2em 0em 2em 0em" rowspacing="3pt" displaystyle="true"><mtr><mtd><mn>2</mn><mo>−</mo><mi>b</mi><mo>=</mo><mn>1</mn></mtd></mtr><mtr><mtd><mn>2</mn><mo>−</mo><mn>1</mn><mo>=</mo><mi>b</mi></mtd></mtr><mtr><mtd><mi>b</mi><mo>=</mo><mn>1</mn></mtd></mtr></mtable></math>

所以这个方程组的解是

<math xmlns="http://www.w3.org/1998/Math/MathML" display="block"><mrow data-mjx-texclass="INNER"><mo data-mjx-texclass="OPEN">{</mo><mtable columnspacing="1em" rowspacing="4pt"><mtr><mtd><mi>a</mi><mo>=</mo><mn>2</mn></mtd></mtr><mtr><mtd><mi>b</mi><mo>=</mo><mn>1</mn></mtd></mtr></mtable><mo data-mjx-texclass="CLOSE" fence="true" stretchy="true" symmetric="true"></mo></mrow></math>

---

### 标准库

<math xmlns="http://www.w3.org/1998/Math/MathML"><mi>A</mi><mo>⋆</mo><mi>B</mi></math>，得

<math xmlns="http://www.w3.org/1998/Math/MathML" display="block"><msub><mi>A</mi><mrow><mo>左</mo></mrow></msub><mo>⋆</mo><msub><mi>B</mi><mrow><mo>左</mo></mrow></msub><mo>=</mo><msub><mi>A</mi><mrow><mo>右</mo></mrow></msub><mo>⋆</mo><msub><mi>B</mi><mrow><mo>右</mo></mrow></msub></math>

此步一般省略，特此标注
