## 二元一次

### 一般形式


将你的式子调整至格式统一

<math xmlns="http://www.w3.org/1998/Math/MathML" display="block"><mi>a</mi><msup><mi>x</mi><mrow><mn>2</mn></mrow></msup><mo>+</mo><mi>b</mi><mi>x</mi><mo>+</mo><mi>c</mi><mo>=</mo><mn>0</mn><mo stretchy="false">(</mo><mi>a</mi><mo>≠</mo><mn>0</mn><mo stretchy="false">)</mo></math>

### 原理

<math xmlns="http://www.w3.org/1998/Math/MathML" display="block"><mtable columnspacing="1em" rowspacing="4pt"><mtr><mtd><msup><mi>a</mi><mrow><mn>2</mn></mrow></msup><mo>=</mo><mi>b</mi></mtd></mtr><mtr><mtd><msub><mi>a</mi><mrow><mn>1</mn></mrow></msub><mo>=</mo><mi>b</mi><mo>，</mo><msub><mi>a</mi><mrow><mn>2</mn></mrow></msub><mo>=</mo><mo>−</mo><mi>b</mi></mtd></mtr></mtable></math>

也可以这样**说**

<math xmlns="http://www.w3.org/1998/Math/MathML" display="block"><mtable columnspacing="1em" rowspacing="4pt"><mtr><mtd><msup><mi>a</mi><mrow><mn>2</mn></mrow></msup><mo>=</mo><mi>b</mi></mtd></mtr><mtr><mtd><mi>a</mi><mo>=</mo><mo>±</mo><msqrt><mi>b</mi></msqrt></mtd></mtr></mtable></math>

---


## 配（完全平）方法

这样写

<math xmlns="http://www.w3.org/1998/Math/MathML" display="block"><mtable columnalign="right left right left right left right left right left right left" columnspacing="0em 2em 0em 2em 0em 2em 0em 2em 0em 2em 0em" rowspacing="3pt" displaystyle="true"><mtr><mtd><msup><mi>x</mi><mrow><mn>2</mn></mrow></msup><mo>+</mo><mstyle scriptlevel="0" displaystyle="false"><mfrac><mi>b</mi><mi>a</mi></mfrac></mstyle><mi>x</mi><mo>=</mo><mstyle scriptlevel="0" displaystyle="false"><mfrac><mi>c</mi><mi>a</mi></mfrac></mstyle></mtd></mtr><mtr><mtd><msup><mi>x</mi><mrow><mn>2</mn></mrow></msup><mo>+</mo><mstyle scriptlevel="0" displaystyle="false"><mfrac><mi>b</mi><mi>a</mi></mfrac></mstyle><mi>x</mi><mo>+</mo><mo stretchy="false">(</mo><mfrac><mi>b</mi><mrow><mn>2</mn><mi>a</mi></mrow></mfrac><msup><mo stretchy="false">)</mo><mrow><mn>2</mn></mrow></msup><mo>=</mo><mstyle scriptlevel="0" displaystyle="false"><mfrac><mi>c</mi><mi>a</mi></mfrac></mstyle><mo>+</mo><mo stretchy="false">(</mo><mfrac><mi>b</mi><mrow><mn>2</mn><mi>a</mi></mrow></mfrac><msup><mo stretchy="false">)</mo><mrow><mn>2</mn></mrow></msup></mtd></mtr><mtr><mtd><mo stretchy="false">(</mo><mi>x</mi><mo>+</mo><mfrac><mi>b</mi><mrow><mn>2</mn><mi>a</mi></mrow></mfrac><msup><mo stretchy="false">)</mo><mrow><mn>2</mn></mrow></msup><mo>=</mo><mstyle scriptlevel="0" displaystyle="false"><mfrac><mi>c</mi><mi>a</mi></mfrac></mstyle><mo>+</mo><mo stretchy="false">(</mo><mfrac><mi>b</mi><mrow><mn>2</mn><mi>a</mi></mrow></mfrac><msup><mo stretchy="false">)</mo><mrow><mn>2</mn></mrow></msup></mtd></mtr><mtr><mtd><mo>∵</mo><mstyle scriptlevel="0" displaystyle="false"><mfrac><mi>c</mi><mi>a</mi></mfrac></mstyle><mo>+</mo><mo stretchy="false">(</mo><mfrac><mi>b</mi><mrow><mn>2</mn><mi>a</mi></mrow></mfrac><msup><mo stretchy="false">)</mo><mrow><mn>2</mn></mrow></msup><mo>&gt;</mo><mn>0</mn></mtd></mtr><mtr><mtd><mo>∴方程有两个不等的实数根</mo></mtd></mtr><mtr><mtd><mi>x</mi><mo>+</mo><mfrac><mi>b</mi><mrow><mn>2</mn><mi>a</mi></mrow></mfrac><mo>=</mo><mo>±</mo><msqrt><mstyle scriptlevel="0" displaystyle="false"><mfrac><mi>c</mi><mi>a</mi></mfrac></mstyle><mo>+</mo><mo stretchy="false">(</mo><mfrac><mi>b</mi><mrow><mn>2</mn><mi>a</mi></mrow></mfrac><msup><mo stretchy="false">)</mo><mrow><mn>2</mn></mrow></msup></msqrt></mtd></mtr><mtr><mtd><mo>∴</mo><mi>x</mi><mo>=</mo><mo>?</mo><mo>或</mo><mi>x</mi><mo>=</mo><mo>?</mo></mtd></mtr><mtr><mtd><mo>∴</mo><msub><mi>x</mi><mrow><mn>1</mn></mrow></msub><mo>=</mo><mo>?</mo><mo>，</mo><msub><mi>x</mi><mrow><mn>2</mn></mrow></msub><mo>=</mo><mo>?</mo></mtd></mtr></mtable></math>

## 公式法

这样写

<math xmlns="http://www.w3.org/1998/Math/MathML" display="block"><mtable columnalign="right left right left right left right left right left right left" columnspacing="0em 2em 0em 2em 0em 2em 0em 2em 0em 2em 0em" rowspacing="3pt" displaystyle="true"><mtr><mtd><mi>a</mi><msup><mi>x</mi><mrow><mn>2</mn></mrow></msup><mo>+</mo><mi>b</mi><mi>x</mi><mo>+</mo><mi>c</mi><mo>=</mo><mn>0</mn></mtd></mtr><mtr><mtd><mo>∵</mo><mi>a</mi><mo>=</mo><mo>?</mo><mo>,</mo><mi>b</mi><mo>=</mo><mo>?</mo><mo>,</mo><mi>c</mi><mo>=</mo><mo>?</mo></mtd></mtr><mtr><mtd><mo>∴</mo><mo>△</mo><mo>=</mo><msup><mi>b</mi><mrow><mn>2</mn></mrow></msup><mo>−</mo><mn>4</mn><mi>a</mi><mi>c</mi><mo>=</mo><mo>?</mo><mo>=</mo><mn>0</mn></mtd></mtr><mtr><mtd><mo>∴方程有两个相等的实数根</mo></mtd></mtr><mtr><mtd><msub><mi>x</mi><mrow><mn>1</mn></mrow></msub><mo>=</mo><msub><mi>x</mi><mrow><mn>2</mn></mrow></msub><mo>=</mo><mfrac><mrow><mo>−</mo><mi>b</mi><mo>±</mo><msqrt><msup><mi>b</mi><mrow><mn>2</mn></mrow></msup><mo>−</mo><mn>4</mn><mi>a</mi><mi>c</mi></msqrt></mrow><mrow><mn>2</mn><mi>a</mi></mrow></mfrac><mo>=</mo><mo>?</mo></mtd></mtr></mtable></math>

## 因式分解法

这样写

<math xmlns="http://www.w3.org/1998/Math/MathML" display="block"><mtable columnalign="right left right left right left right left right left right left" columnspacing="0em 2em 0em 2em 0em 2em 0em 2em 0em 2em 0em" rowspacing="3pt" displaystyle="true"><mtr><mtd><mi>A</mi><mo>×</mo><mi>B</mi><mo>=</mo><mn>0</mn></mtd></mtr><mtr><mtd><mo>∴</mo><mi>A</mi><mo>=</mo><mn>0</mn><mo>或</mo><mi>B</mi><mo>=</mo><mn>0</mn></mtd></mtr><mtr><mtd><mo>∴</mo><msub><mi>x</mi><mrow><mn>1</mn></mrow></msub><mo>=</mo><mo>?</mo><mo>，</mo><msub><mi>x</mi><mrow><mn>2</mn></mrow></msub><mo>=</mo><mo>?</mo></mtd></mtr></mtable></math>
